Half of completeness theorem

theories/Core/Completeness/LogicalRelation/Definitions.v
@@ -4,100 +4,101 @@ From McPTS.Core Require Import Base.
 From McPTS.Core.Semantic Require Export PER.
 Import Domain_Notations.
 
-Inductive rel_exp {P : PtsSig} M ρ M' ρ' (R : relation (domain P)) : Prop :=
-| mk_rel_exp : forall m m', {{ ⟦ M ⟧ ρ ↘ m }} -> {{ ⟦ M' ⟧ ρ' ↘ m' }} -> {{ Dom m ≈ m' ∈ R }} -> rel_exp M ρ M' ρ' R.
+Inductive rel_exp {P : PtsSig} Δ M ρ M' ρ' (R : relation (domain P)) : Prop :=
+| mk_rel_exp : forall m m', {{ Δ ▶ ⟦ M ⟧ ρ ↘ m }} -> {{ Δ ▶ ⟦ M' ⟧ ρ' ↘ m' }} -> {{ Dom m ≈ m' ∈ R }} -> rel_exp Δ M ρ M' ρ' R.
 #[global]
-Arguments mk_rel_exp {_ _ _ _ _ _}.
+Arguments mk_rel_exp {_ _ _ _ _ _ _}.
 #[export]
 Hint Constructors rel_exp : mcpts.
 
-Definition rel_exp_under_ctx {P : PtsSig} (pred_P : PredicativeSig P) (Γ : ctx P) A M M' :=
+(* Definition rel_exp_under_ctx {P : PtsSig} (pred_P : PredicativeSig P) (Δ : gctx P) Γ A M M' := *)
+(*   exists env_rel, *)
+(*     {{ EF Γ ≈ Γ ∈ per_ctx_env Δ pred_P ↘ env_rel }} /\ *)
+(*       exists s, *)
+(*       forall ρ ρ' (equiv_ρ_ρ' : {{ Dom ρ ≈ ρ' ∈ env_rel }}), *)
+(*       exists (elem_rel : relation (domain P)), *)
+(*         rel_typ pred_P s A ρ A ρ' elem_rel /\ rel_exp M ρ M' ρ' elem_rel. *)
+
+(* Definition valid_exp_under_ctx {P : PtsSig} (pred_P : PredicativeSig P) Γ A M := rel_exp_under_ctx pred_P Γ A M M. *)
+(* #[global] *)
+(* Arguments valid_exp_under_ctx {_} _ _ _ _ /. *)
+(* #[export] *)
+(* Hint Transparent valid_exp_under_ctx : mcpts. *)
+(* #[export] *)
+(* Hint Unfold valid_exp_under_ctx : mcpts. *)
+
+
+Definition rel_exp_under_ctx_unsorted {P} (pred_P : PredicativeSig P) (Δ : gctx P) Γ A M M' :=
   exists env_rel,
-    {{ EF Γ ≈ Γ ∈ per_ctx_env pred_P ↘ env_rel }} /\
-      exists s,
+    {{ EF Γ ≈ Γ ∈ per_ctx_env pred_P Δ ↘ env_rel }} /\
       forall ρ ρ' (equiv_ρ_ρ' : {{ Dom ρ ≈ ρ' ∈ env_rel }}),
       exists (elem_rel : relation (domain P)),
-        rel_typ pred_P s A ρ A ρ' elem_rel /\ rel_exp M ρ M' ρ' elem_rel.
+        rel_typ_unsorted pred_P Δ A ρ A ρ' elem_rel /\ rel_exp Δ M ρ M' ρ' elem_rel.
 
-Definition valid_exp_under_ctx {P : PtsSig} (pred_P : PredicativeSig P) Γ A M := rel_exp_under_ctx pred_P Γ A M M.
+Definition valid_exp_under_ctx_unsorted {P : PtsSig} (pred_P : PredicativeSig P) Δ Γ A M := rel_exp_under_ctx_unsorted pred_P Δ Γ A M M.
 #[global]
-Arguments valid_exp_under_ctx {_} _ _ _ _ /.
-#[export]
-Hint Transparent valid_exp_under_ctx : mcpts.
-#[export]
-Hint Unfold valid_exp_under_ctx : mcpts.
-
-
-Definition rel_exp_under_ctx_unsorted {P} (pred_P : PredicativeSig P) (Γ : ctx P) A M M' :=
-  exists env_rel,
-    {{ EF Γ ≈ Γ ∈ per_ctx_env pred_P ↘ env_rel }} /\
-      forall ρ ρ' (equiv_ρ_ρ' : {{ Dom ρ ≈ ρ' ∈ env_rel }}),
-      exists (elem_rel : relation (domain P)),
-        rel_typ_unsorted pred_P A ρ A ρ' elem_rel /\ rel_exp M ρ M' ρ' elem_rel.
-
-Definition valid_exp_under_ctx_unsorted {P : PtsSig} (pred_P : PredicativeSig P) Γ A M := rel_exp_under_ctx_unsorted pred_P Γ A M M.
-#[global]
-Arguments valid_exp_under_ctx_unsorted {_} _ _ _ _ /.
+Arguments valid_exp_under_ctx_unsorted {_} _ _ _ _ _ /.
 #[export]
 Hint Transparent valid_exp_under_ctx_unsorted : mcpts.
 #[export]
 Hint Unfold valid_exp_under_ctx_unsorted : mcpts.
 
 
-Definition rel_typ_under_ctx {P} (pred_P : PredicativeSig P) (Γ : ctx P) A A' :=
+Definition rel_typ_under_ctx {P} (pred_P : PredicativeSig P) (Δ : gctx P) Γ A A' :=
   exists env_rel,
-    {{ EF Γ ≈ Γ ∈ per_ctx_env pred_P ↘ env_rel }} /\
+    {{ EF Γ ≈ Γ ∈ per_ctx_env pred_P Δ ↘ env_rel }} /\
       forall ρ ρ' (equiv_ρ_ρ' : {{ Dom ρ ≈ ρ' ∈ env_rel }}),
       exists (elem_rel : relation (domain P)),
-        rel_typ_unsorted pred_P A ρ A' ρ' elem_rel.
+        rel_typ_unsorted pred_P Δ A ρ A' ρ' elem_rel.
 
-Definition valid_typ_under_ctx {P} {pred_P : PredicativeSig P} Γ A := rel_typ_under_ctx pred_P Γ A A.
+Definition valid_typ_under_ctx {P} (pred_P : PredicativeSig P) Δ Γ A := rel_typ_under_ctx pred_P Δ Γ A A.
 #[global]
-Arguments valid_typ_under_ctx {_} _ _ _ /.
+Arguments valid_typ_under_ctx {_} _ _ _ _ /.
 #[export]
 Hint Transparent valid_typ_under_ctx : mcpts.
 #[export]
 Hint Unfold valid_typ_under_ctx : mcpts.
 
 
-Inductive rel_sub {P : PtsSig} σ ρ σ' ρ' (R : relation (env P)) : Prop :=
-| mk_rel_sub : forall ρσ ρ'σ', {{ ⟦ σ ⟧s ρ ↘ ρσ }} -> {{ ⟦ σ' ⟧s ρ' ↘ ρ'σ' }} -> {{ Dom ρσ ≈ ρ'σ' ∈ R }} -> rel_sub σ ρ σ' ρ' R.
+Inductive rel_sub {P : PtsSig} Δ σ ρ σ' ρ' (R : relation (env P)) : Prop :=
+| mk_rel_sub : forall ρσ ρ'σ', {{ Δ ▶ ⟦ σ ⟧s ρ ↘ ρσ }} -> {{ Δ ▶ ⟦ σ' ⟧s ρ' ↘ ρ'σ' }} -> {{ Dom ρσ ≈ ρ'σ' ∈ R }} -> rel_sub Δ σ ρ σ' ρ' R.
 #[global]
-Arguments mk_rel_sub {_ _ _ _ _ _ _}.
+Arguments mk_rel_sub {_ _ _ _ _ _ _ _}.
 #[export]
 Hint Constructors rel_sub : mcpts.
 
-Definition rel_sub_under_ctx {P : PtsSig} (pred_P : PredicativeSig P) Γ Δ σ σ' :=
+Definition rel_sub_under_ctx {P : PtsSig} (pred_P : PredicativeSig P) Δ Γ Γ' σ σ' :=
   exists env_rel,
-    {{ EF Γ ≈ Γ ∈ per_ctx_env pred_P ↘ env_rel }} /\
+    {{ EF Γ ≈ Γ ∈ per_ctx_env pred_P Δ ↘ env_rel }} /\
       exists env_rel',
-        {{ EF Δ ≈ Δ ∈ per_ctx_env pred_P ↘ env_rel' }} /\
+        {{ EF Γ' ≈ Γ' ∈ per_ctx_env pred_P Δ ↘ env_rel' }} /\
           (forall ρ ρ' (equiv_ρ_ρ' : {{ Dom ρ ≈ ρ' ∈ env_rel }}),
-              rel_sub σ ρ σ' ρ' env_rel').
+              rel_sub Δ σ ρ σ' ρ' env_rel').
 
-Definition valid_sub_under_ctx {P : PtsSig} (pred_P : PredicativeSig P) Γ Δ σ := rel_sub_under_ctx pred_P Γ Δ σ σ.
+Definition valid_sub_under_ctx {P : PtsSig} (pred_P : PredicativeSig P) Δ Γ Γ' σ := rel_sub_under_ctx pred_P Δ Γ Γ' σ σ.
 #[global]
-Arguments valid_sub_under_ctx {_} _ _ _ _ /.
+Arguments valid_sub_under_ctx {_} _ _ _ _ _ /.
 #[export]
 Hint Transparent valid_sub_under_ctx : mcpts.
 #[export]
 Hint Unfold valid_sub_under_ctx : mcpts.
 
-Definition subtyp_under_ctx {P : PtsSig} (pred_P : PredicativeSig P) (Γ : ctx P) M M' :=
+Definition subtyp_under_ctx {P : PtsSig} (pred_P : PredicativeSig P) Δ Γ M M' :=
   exists env_rel,
-    {{ EF Γ ≈ Γ ∈ per_ctx_env pred_P ↘ env_rel }} /\
+    {{ EF Γ ≈ Γ ∈ per_ctx_env pred_P Δ ↘ env_rel }} /\
       forall ρ ρ' (equiv_ρ_ρ' : {{ Dom ρ ≈ ρ' ∈ env_rel }}),
-        exists R R', rel_typ_unsorted pred_P M ρ M ρ' R /\ rel_typ_unsorted pred_P M' ρ M' ρ' R' /\ rel_exp M ρ M' ρ' (per_subtyp pred_P).
+        exists R R', rel_typ_unsorted pred_P Δ M ρ M ρ' R /\ rel_typ_unsorted pred_P Δ M' ρ M' ρ' R' /\ rel_exp Δ M ρ M' ρ' (per_subtyp pred_P Δ).
                                   
-           
-Notation "⟪ pred_P ⟫ ⊨ Γ ≈ Γ'" := (per_ctx pred_P Γ Γ')  (in custom judg at level 80, pred_P constr, Γ custom exp, Γ' custom exp).
-Notation "⟪ pred_P ⟫ ⊨ Γ" := (valid_ctx pred_P Γ) (in custom judg at level 80, pred_P constr, Γ custom exp).
-Notation "⟪ pred_P ⟫ Γ ⊨ M ≈ M' : A" := (rel_exp_under_ctx pred_P Γ A M M') (in custom judg at level 80, pred_P constr, Γ custom exp, M custom exp, M' custom exp, A custom exp).
-Notation "⟪ pred_P ⟫ Γ ⊨ M : A" := (valid_exp_under_ctx pred_P Γ A M) (in custom judg at level 80, pred_P constr, Γ custom exp, M custom exp, A custom exp).
-Notation "⟪ pred_P ⟫ Γ ⊨u M ≈ M' : A" := (rel_exp_under_ctx_unsorted pred_P Γ A M M') (in custom judg at level 80, pred_P constr, Γ custom exp, M custom exp, M' custom exp, A custom exp).
-Notation "⟪ pred_P ⟫ Γ ⊨u M : A" := (valid_exp_under_ctx_unsorted pred_P Γ A M) (in custom judg at level 80, pred_P constr, Γ custom exp, M custom exp, A custom exp).
-Notation "⟪ pred_P ⟫ Γ ⊨ A ≈ A'" := (rel_typ_under_ctx pred_P Γ A A') (in custom judg at level 80, pred_P constr, Γ custom exp, A custom exp, A' custom exp).
-Notation "⟪ pred_P ⟫ Γ ⊨ A" := (valid_typ_under_ctx pred_P Γ A) (in custom judg at level 80, pred_P constr, Γ custom exp, A custom exp).
-Notation "⟪ pred_P ⟫ Γ ⊨s σ ≈ σ' : Δ" := (rel_sub_under_ctx pred_P Γ Δ σ σ') (in custom judg at level 80, pred_P constr, Γ custom exp, σ custom exp, σ' custom exp, Δ custom exp).
-Notation "⟪ pred_P ⟫ Γ ⊨s σ : Δ" := (valid_sub_under_ctx pred_P Γ Δ σ) (in custom judg at level 80, pred_P constr, Γ custom exp, σ custom exp, Δ custom exp).
-Notation "⟪ pred_P ⟫ Γ ⊨ M ⊆ M'" := (subtyp_under_ctx pred_P Γ M M') (in custom judg at level 80, pred_P constr, Γ custom exp, M custom exp, M' custom exp).
+Notation "⟪ pred_P ⟫ ▶ Δ ≈ Δ'" := (per_gctx pred_P Δ Δ') (in custom judg at level 80, pred_P constr, Δ custom exp, Δ' custom exp).
+Notation "⟪ pred_P ⟫ ▶ Δ" := (per_gctx pred_P Δ Δ) (in custom judg at level 80, pred_P constr, Δ custom exp).
+Notation "⟪ pred_P ⟫ Δ ▶ Γ ≈ Γ'" := (per_ctx pred_P Δ Γ Γ')  (in custom judg at level 80, pred_P constr, Δ custom exp, Γ custom exp, Γ' custom exp).
+Notation "⟪ pred_P ⟫ Δ ▶ Γ" := (valid_ctx pred_P Δ Γ) (in custom judg at level 80, pred_P constr, Δ custom exp, Γ custom exp).
+(* Notation "⟪ pred_P ⟫ Δ ▶ Γ ⊨ M ≈ M' : A" := (rel_exp_under_ctx pred_P Δ Γ A M M') (in custom judg at level 80, pred_P constr, Δ custom exp, Γ custom exp, M custom exp, M' custom exp, A custom exp). *)
+(* Notation "⟪ pred_P ⟫ Γ ⊨ M : A" := (valid_exp_under_ctx pred_P Γ A M) (in custom judg at level 80, pred_P constr, Γ custom exp, M custom exp, A custom exp). *)
+Notation "⟪ pred_P ⟫ Δ ▶ Γ ⊨u M ≈ M' : A" := (rel_exp_under_ctx_unsorted pred_P Δ Γ A M M') (in custom judg at level 80, pred_P constr, Δ custom exp, Γ custom exp, M custom exp, M' custom exp, A custom exp).
+Notation "⟪ pred_P ⟫ Δ ▶ Γ ⊨u M : A" := (valid_exp_under_ctx_unsorted pred_P Δ Γ A M) (in custom judg at level 80, pred_P constr, Δ custom exp, Γ custom exp, M custom exp, A custom exp).
+Notation "⟪ pred_P ⟫ Δ ▶ Γ ⊨ A ≈ A'" := (rel_typ_under_ctx pred_P Δ Γ A A') (in custom judg at level 80, pred_P constr, Δ custom exp, Γ custom exp, A custom exp, A' custom exp).
+Notation "⟪ pred_P ⟫ Δ ▶ Γ ⊨ A" := (valid_typ_under_ctx pred_P Δ Γ A) (in custom judg at level 80, pred_P constr, Δ custom exp, Γ custom exp, A custom exp).
+Notation "⟪ pred_P ⟫ Δ ▶ Γ ⊨s σ ≈ σ' : Γ'" := (rel_sub_under_ctx pred_P Δ Γ Γ' σ σ') (in custom judg at level 80, pred_P constr, Δ custom exp, Γ custom exp, σ custom exp, σ' custom exp, Γ' custom exp).
+Notation "⟪ pred_P ⟫ Δ ▶ Γ ⊨s σ : Γ'" := (valid_sub_under_ctx pred_P Δ Γ Γ' σ) (in custom judg at level 80, pred_P constr, Δ custom exp, Γ custom exp, σ custom exp, Γ' custom exp).
+Notation "⟪ pred_P ⟫ Δ ▶ Γ ⊨ M ⊆ M'" := (subtyp_under_ctx pred_P Δ Γ M M') (in custom judg at level 80, pred_P constr, Δ custom exp, Γ custom exp, M custom exp, M' custom exp).
