theories/Core/Completeness/ContextCases.v
@@ -2,32 +2,103 @@ From Coq Require Import Morphisms_Relations.
 
 From McPTS Require Import PtsSignature LibTactics.
 From McPTS.Core Require Import Base.
+From McPTS.Core.Syntactic Require Import System.
 From McPTS.Core.Completeness Require Import LogicalRelation SortCases.
 Import Domain_Notations.
 
-Proposition valid_ctx_empty {P : PtsSig} {pred_P : PredicativeSig P} :
-  {{ ⟪ pred_P ⟫ ⊨ ⋅ }}.
+(** ** Global context cases *)
+Proposition valid_gctx_empty {P} {pred_P : PredicativeSig P} :
+  {{ ⟪ pred_P ⟫ ▶ ⋅ }}.
+Proof. mauto 2. Qed.
+
+Proposition rel_gctx_empty {P} {pred_P : PredicativeSig P} :
+  {{ ⟪ pred_P ⟫ ▶ ⋅ ≈ ⋅ }}.
+Proof. mauto 2. Qed.
+
+Proposition rel_gctx_subtyp_empty {P} {pred_P : PredicativeSig P} :
+  {{ SubG ⋅ <: ⋅ ∈ per_gctx_subtyp pred_P }}.
+Proof. econstructor. Qed.
+
+#[export]
+Hint Resolve valid_gctx_empty rel_gctx_empty rel_gctx_subtyp_empty : mcpts.
+    
+Proposition rel_gctx_extend {P} {pred_P : PredicativeSig P} : forall {Δ Δ' x A A'},
+    {{ ⟪ pred_P ⟫ ▶ Δ ≈ Δ' }} ->
+    {{ ⟪ pred_P ⟫ Δ ▶ ⋅ ⊨ A ≈ A' }} ->
+    {{ ⟪ pred_P ⟫ Δ' ▶ ⋅ ⊨ A ≈ A' }} ->
+    {{ `#x ∉ Δ }} -> 
+    {{ ⟪ pred_P ⟫ ▶ Δ, x:A ≈ Δ', x:A' }}.
 Proof.
-  do 2 econstructor.
+  intros * ? [env_rel []] [env_rel' []] ?.
+  inversion H0; subst.
+  inversion H2; subst.
+  assert (env_rel d{{{ ⋅ }}} d{{{ ⋅ }}}) as equiv_env_rel by (apply_relation_equivalence; mauto 2).
+  assert (env_rel' d{{{ ⋅ }}} d{{{ ⋅ }}}) as equiv_env_rel' by intuition. 
+  pose proof (H1 _ _ equiv_env_rel) as [elem_rel].
+  pose proof (H3 _ _ equiv_env_rel') as [elem_rel'].
+  econstructor; mauto 2; try reflexivity.
+Qed.
+
+Proposition valid_gctx_extend {P} {pred_P : PredicativeSig P} : forall {Δ x A},
+    {{ ⟪ pred_P ⟫ ▶ Δ }} ->
+    {{ ⟪ pred_P ⟫ Δ ▶ ⋅ ⊨ A }} ->
+    {{ `#x ∉ Δ }} -> 
+    {{ ⟪ pred_P ⟫ ▶ Δ, x:A }}.
+Proof.
+  intros.
+  eapply rel_gctx_extend; mauto 2.
+Qed.
+
+Proposition rel_gctx_subtyp_extend {P} {pred_P : PredicativeSig P} : forall {Δ Δ' x A A'},
+    {{ SubG Δ <: Δ' ∈ per_gctx_subtyp pred_P }} ->
+    {{ ⟪ pred_P ⟫ Δ ▶ ⋅ ⊨ A }} ->
+    {{ ⟪ pred_P ⟫ Δ' ▶ ⋅ ⊨ A' }} ->
+    {{ ⟪ pred_P ⟫ Δ ▶ ⋅ ⊨ A ⊆ A' }} ->
+    {{ `#x ∉ Δ }} ->
+    {{ SubG Δ, x:A <: Δ', x:A' ∈ per_gctx_subtyp pred_P }}.
+Proof.
+  intros * ? [env_rel []] [env_rel' []] [env_rel'' []] ?.
+  invert_per_ctx_envs.
+  apply_relation_equivalence.
+  specialize (H1 d{{{ ⋅ }}} d{{{ ⋅ }}} ltac:(auto)) as [elem_rel].
+  specialize (H3 d{{{ ⋅ }}} d{{{ ⋅ }}} ltac:(auto)) as [elem_rel'].
+  specialize (H5 d{{{ ⋅ }}} d{{{ ⋅ }}} ltac:(auto)) as [R [R' [? []]]].
+
+  destruct_rel_typ_unsorted.
+  destruct_by_head (@rel_exp).
+  econstructor; mauto 2.
+Qed.
+
+#[export]
+Hint Resolve rel_gctx_extend valid_gctx_extend rel_gctx_subtyp_extend : mcpts.
+
+
+(** ** Local context cases *)
+Proposition valid_ctx_empty {P : PtsSig} {pred_P : PredicativeSig P} : forall {Δ},
+    {{ ⟪ pred_P ⟫ ▶ Δ }} -> 
+    {{ ⟪ pred_P ⟫ Δ ▶ ⋅ }}.
+Proof.
+  do 2 econstructor; mauto 2.
   apply Equivalence_Reflexive.
 Qed.
 
-#[export]
-Hint Resolve valid_ctx_empty : mcpts.
-
-Lemma rel_ctx_empty {P} {pred_P : PredicativeSig P} :
-  {{ ⟪ pred_P ⟫ ⊨ ⋅ ≈ ⋅ }}.
+Lemma rel_ctx_empty {P} {pred_P : PredicativeSig P} : forall {Δ},
+  {{ ⟪ pred_P ⟫ ▶ Δ }} -> 
+  {{ ⟪ pred_P ⟫ Δ ▶ ⋅ ≈ ⋅ }}.
 Proof.
-  apply valid_ctx_empty.
+  do 2 econstructor; mauto 2.
+  apply Equivalence_Reflexive.
 Qed.
 
-#[export]
-Hint Resolve rel_ctx_empty : mcpts.
 
-Lemma rel_ctx_extend {P : PtsSig} {pred_P : PredicativeSig P} : forall {Γ Γ' A A'},
-    {{ ⟪ pred_P ⟫ ⊨ Γ ≈ Γ' }} ->
-    {{ ⟪ pred_P ⟫ Γ ⊨ A ≈ A' }} ->
-    {{ ⟪ pred_P ⟫ ⊨ Γ, A ≈ Γ', A' }}.
+#[export]
+Hint Resolve valid_ctx_empty rel_ctx_empty : mcpts.
+
+
+Lemma rel_ctx_extend {P : PtsSig} {pred_P : PredicativeSig P} : forall {Δ Γ Γ' A A'},
+    {{ ⟪ pred_P ⟫ Δ ▶ Γ ≈ Γ' }} ->
+    {{ ⟪ pred_P ⟫ Δ ▶ Γ ⊨ A ≈ A' }} ->
+    {{ ⟪ pred_P ⟫ Δ ▶ Γ, A ≈ Γ', A' }}.
 Proof with intuition.
   intros * [] [env_relΓ]%rel_exp_of_typ_unsorted_inversion1.
   pose env_relΓ.
@@ -37,7 +108,7 @@ Proof with intuition.
   per_ctx_env_econstructor; eauto.
   - instantiate (1 := fun ρ ρ' (equiv_ρ_ρ' : env_relΓ ρ ρ') m m' =>
                         forall R,
-                          rel_typ_unsorted pred_P A ρ A' ρ' R ->
+                          rel_typ_unsorted pred_P Δ A ρ A' ρ' R ->
                           R m m').
     intros.
     (on_all_hyp: destruct_rel_by_assumption env_relΓ).
@@ -45,50 +116,50 @@ Proof with intuition.
     econstructor; eauto.
     apply -> per_typ_elem_morphism_iff; eauto.
     split; intros; destruct_by_head (@rel_typ_unsorted P); handle_per_typ_elem_irrel...
-    assert (rel_typ_unsorted pred_P A ρ A' ρ' elem_relA) by mauto.
+    assert (rel_typ_unsorted pred_P Δ A ρ A' ρ' elem_relA) by mauto.
     intuition.
   - apply Equivalence_Reflexive.
 Qed.
 
-Lemma rel_ctx_extend_het {P} {pred_P : PredicativeSig P} : forall {Γ Δ A A'},
-    {{ ⟪ pred_P ⟫ ⊨ Γ ≈ Δ }} ->
-    {{ ⟪ pred_P ⟫ Γ ⊨ A }} ->
-    {{ ⟪ pred_P ⟫ Γ ⊨ A' }} ->
-    {{ ⟪ pred_P ⟫ Δ ⊨ A }} ->
-    {{ ⟪ pred_P ⟫ Δ ⊨ A' }} ->
-    {{ ⟪ pred_P ⟫ Γ ⊨ A ≈ A' }} ->
-    {{ ⟪ pred_P ⟫ Δ ⊨ A ≈ A' }} ->
-    {{ ⟪ pred_P ⟫ ⊨ Γ, A ≈ Δ, A' }}.
-Proof.
-  intros * [] [env_relΓ]%rel_exp_of_typ_unsorted_inversion1 []%rel_exp_of_typ_unsorted_inversion1
-             [env_relΔ]%rel_exp_of_typ_unsorted_inversion1 []%rel_exp_of_typ_unsorted_inversion1
-             []%rel_exp_of_typ_unsorted_inversion1 []%rel_exp_of_typ_unsorted_inversion1.
-  destruct_conjs.
-  handle_per_ctx_env_irrel.
-  eexists.
-  per_ctx_env_econstructor; eauto.
-  - instantiate (1 := fun ρ ρ' (equiv_ρ_ρ' : x ρ ρ') m m' =>
-                        forall R,
-                          rel_typ_unsorted pred_P A ρ A' ρ' R ->
-                          R m m').
-    intros.
-    (on_all_hyp: destruct_rel_by_assumption x).
-    match_by_head (@per_typ P) ltac:(fun H => destruct H as [elem_relA]).
-    econstructor; eauto.
-    destruct_by_head (@per_typ P).
-    simplify_evals.
-    handle_per_typ_elem_irrel.
-    apply -> per_typ_elem_morphism_iff; [apply H2 | reflexivity | reflexivity |].
-    split; intros; destruct_by_head (@rel_typ_unsorted P); handle_per_typ_elem_irrel;
-      assert (rel_typ_unsorted pred_P A ρ A' ρ' x1) by mauto;
-      intuition.
+(* Lemma rel_ctx_extend_het {P} {pred_P : PredicativeSig P} : forall {Γ Δ A A'}, *)
+(*     {{ ⟪ pred_P ⟫ ⊨ Γ ≈ Δ }} -> *)
+(*     {{ ⟪ pred_P ⟫ Γ ⊨ A }} -> *)
+(*     {{ ⟪ pred_P ⟫ Γ ⊨ A' }} -> *)
+(*     {{ ⟪ pred_P ⟫ Δ ⊨ A }} -> *)
+(*     {{ ⟪ pred_P ⟫ Δ ⊨ A' }} -> *)
+(*     {{ ⟪ pred_P ⟫ Γ ⊨ A ≈ A' }} -> *)
+(*     {{ ⟪ pred_P ⟫ Δ ⊨ A ≈ A' }} -> *)
+(*     {{ ⟪ pred_P ⟫ ⊨ Γ, A ≈ Δ, A' }}. *)
+(* Proof. *)
+(*   intros * [] [env_relΓ]%rel_exp_of_typ_unsorted_inversion1 []%rel_exp_of_typ_unsorted_inversion1 *)
+(*              [env_relΔ]%rel_exp_of_typ_unsorted_inversion1 []%rel_exp_of_typ_unsorted_inversion1 *)
+(*              []%rel_exp_of_typ_unsorted_inversion1 []%rel_exp_of_typ_unsorted_inversion1. *)
+(*   destruct_conjs. *)
+(*   handle_per_ctx_env_irrel. *)
+(*   eexists. *)
+(*   per_ctx_env_econstructor; eauto. *)
+(*   - instantiate (1 := fun ρ ρ' (equiv_ρ_ρ' : x ρ ρ') m m' => *)
+(*                         forall R, *)
+(*                           rel_typ_unsorted pred_P A ρ A' ρ' R -> *)
+(*                           R m m'). *)
+(*     intros. *)
+(*     (on_all_hyp: destruct_rel_by_assumption x). *)
+(*     match_by_head (@per_typ P) ltac:(fun H => destruct H as [elem_relA]). *)
+(*     econstructor; eauto. *)
+(*     destruct_by_head (@per_typ P). *)
+(*     simplify_evals. *)
+(*     handle_per_typ_elem_irrel. *)
+(*     apply -> per_typ_elem_morphism_iff; [apply H2 | reflexivity | reflexivity |]. *)
+(*     split; intros; destruct_by_head (@rel_typ_unsorted P); handle_per_typ_elem_irrel; *)
+(*       assert (rel_typ_unsorted pred_P A ρ A' ρ' x1) by mauto; *)
+(*       intuition. *)
 
-  - apply Equivalence_Reflexive.
-Qed.
+(*   - apply Equivalence_Reflexive. *)
+(* Qed. *)
 
-Lemma rel_ctx_extend' {P : PtsSig} {pred_P : PredicativeSig P} : forall {Γ A},
-    {{ ⟪ pred_P ⟫ Γ ⊨ A }} ->
-    {{ ⟪ pred_P ⟫ ⊨ Γ, A }}.
+Lemma valid_ctx_extend {P : PtsSig} {pred_P : PredicativeSig P} : forall {Δ Γ A},
+    {{ ⟪ pred_P ⟫ Δ ▶ Γ ⊨ A }} ->
+    {{ ⟪ pred_P ⟫ Δ ▶ Γ, A }}.
 Proof.
   intros.
   eapply rel_ctx_extend; eauto.
@@ -97,20 +168,21 @@ Proof.
 Qed.
 
 #[export]
-Hint Resolve rel_ctx_extend rel_ctx_extend_het rel_ctx_extend' : mcpts.
+Hint Resolve rel_ctx_extend valid_ctx_extend : mcpts.
 
-Lemma rel_ctx_sub_empty {P : PtsSig} {pred_P : PredicativeSig P} :
-  {{⟪ pred_P ⟫ SubE ⋅ <: ⋅ }}.
+Lemma rel_ctx_sub_empty {P : PtsSig} {pred_P : PredicativeSig P} : forall {Δ},
+    {{ ⟪ pred_P ⟫ ▶ Δ }} -> 
+    {{ SubC ⋅ <: ⋅ ∈ per_ctx_subtyp pred_P Δ }}.
 Proof. mauto. Qed.
 
-Lemma rel_ctx_sub_extend {P : PtsSig} {pred_P : PredicativeSig P} : forall (Γ : ctx P) Δ A A',
-  {{ ⟪ pred_P ⟫ SubE Γ <: Δ }} ->
-  {{ ⟪ pred_P ⟫ Γ ⊨ A }} ->
-  {{ ⟪ pred_P ⟫ Δ ⊨ A' }} ->
-  {{ ⟪ pred_P ⟫ Γ ⊨ A ⊆ A' }} ->
-  {{ ⟪ pred_P ⟫ SubE Γ , A <: Δ , A' }}.
+Lemma rel_ctx_sub_extend {P : PtsSig} {pred_P : PredicativeSig P} : forall Δ Γ Γ' A A',
+  {{ SubC Γ <: Γ' ∈ per_ctx_subtyp pred_P Δ }} ->
+  {{ ⟪ pred_P ⟫ Δ ▶ Γ ⊨ A }} ->
+  {{ ⟪ pred_P ⟫ Δ ▶ Γ' ⊨ A' }} ->
+  {{ ⟪ pred_P ⟫ Δ ▶ Γ ⊨ A ⊆ A' }} ->
+  {{ SubC Γ , A <: Γ' , A' ∈ per_ctx_subtyp pred_P Δ }}.
 Proof.
-  intros * ? []%rel_ctx_extend' []%rel_ctx_extend' [env_relΓ].
+  intros * ? []%valid_ctx_extend []%valid_ctx_extend [env_relΓ].
   pose env_relΓ.
   destruct_conjs.
   
