theories/Core/Completeness/GlobalContextCases.v
@@ -1,0 +1,11 @@
+From Coq Require Import Morphisms_Relations.
+
+From McPTS Require Import PtsSignature LibTactics.
+From McPTS.Core Require Import Base.
+From McPTS.Core.Completeness Require Import LogicalRelation SortCases.
+Import Domain_Notations.
+
+Proposition valid_gctx_empty {P} {pred_P : PredicativeSig P} :
+  {{ ⟪ pred_P ⟫ ▶ ⋅ }}.
+Proof. mauto 2. Qed.
+  
