theories/Core/Completeness/LogicalRelation/Lemmas.v
@@ -5,33 +5,33 @@ From McPTS.Core Require Import Base.
 From McPTS.Core.Completeness.LogicalRelation Require Import Definitions Tactics.
 Import Domain_Notations.
 
-Add Parametric Morphism {P : PtsSig} M ρ M' ρ' : (rel_exp M ρ M' ρ')
+Add Parametric Morphism {P : PtsSig} Δ M ρ M' ρ' : (rel_exp Δ M ρ M' ρ')
     with signature (@relation_equivalence (domain P)) ==> iff as rel_exp_morphism.
 Proof.
   intros R R' HRR'.
   split; intros []; econstructor; intuition.
 Qed.
 
-Add Parametric Morphism {P : PtsSig} σ ρ σ' ρ' : (rel_sub σ ρ σ' ρ')
+Add Parametric Morphism {P : PtsSig} Δ σ ρ σ' ρ' : (rel_sub Δ σ ρ σ' ρ')
     with signature (@relation_equivalence (env P)) ==> iff as rel_sub_morphism.
 Proof.
   intros R R' HRR'.
   split; intros []; econstructor; intuition.
 Qed.
 
-Lemma rel_exp_implies_rel_typ {P : PtsSig} {pred_P : PredicativeSig P} : forall {s A ρ A' ρ'},
-    rel_exp A ρ A' ρ' (per_sort pred_P s) ->
-    exists R, rel_typ pred_P s A ρ A' ρ' R.
-Proof.
-  intros.
-  destruct_by_head (@rel_exp P).
-  destruct_by_head (@per_sort P).
-  mauto.
-Qed.
+(* Lemma rel_exp_implies_rel_typ {P : PtsSig} {pred_P : PredicativeSig P} : forall {Δ s A ρ A' ρ'}, *)
+(*     rel_exp Δ A ρ A' ρ' (per_sort pred_P Δ s) -> *)
+(*     exists R, rel_typ pred_P Δ s A ρ A' ρ' R. *)
+(* Proof. *)
+(*   intros. *)
+(*   destruct_by_head (@rel_exp P). *)
+(*   destruct_by_head (@per_sort P). *)
+(*   mauto. *)
+(* Qed. *)
 
-Lemma rel_exp_implies_rel_typ_unsorted {P} {pred_P : PredicativeSig P} : forall {A ρ A' ρ'},
-    rel_exp A ρ A' ρ' (per_typ pred_P) ->
-    exists R, rel_typ_unsorted pred_P A ρ A' ρ' R.
+Lemma rel_exp_implies_rel_typ_unsorted {P} {pred_P : PredicativeSig P} : forall {Δ A ρ A' ρ'},
+    rel_exp Δ A ρ A' ρ' (per_typ pred_P Δ) ->
+    exists R, rel_typ_unsorted pred_P Δ A ρ A' ρ' R.
 Proof.
   intros.
   destruct_by_head (@rel_exp P).
@@ -40,20 +40,20 @@ Proof.
 Qed.
 
 #[export]
-Hint Resolve rel_exp_implies_rel_typ rel_exp_implies_rel_typ_unsorted : mcpts.
+Hint Resolve rel_exp_implies_rel_typ_unsorted : mcpts.
 
-Lemma rel_typ_implies_rel_exp {P : PtsSig} {pred_P : PredicativeSig P} : forall {s A ρ A' ρ' R},
-    rel_typ pred_P s A ρ A' ρ' R ->
-    rel_exp A ρ A' ρ' (per_sort pred_P s).
-Proof.
-  intros.
-  destruct_by_head (@rel_typ P).
-  mauto.
-Qed.
+(* Lemma rel_typ_implies_rel_exp {P : PtsSig} {pred_P : PredicativeSig P} : forall {s A ρ A' ρ' R}, *)
+(*     rel_typ pred_P s A ρ A' ρ' R -> *)
+(*     rel_exp A ρ A' ρ' (per_sort pred_P s). *)
+(* Proof. *)
+(*   intros. *)
+(*   destruct_by_head (@rel_typ P). *)
+(*   mauto. *)
+(* Qed. *)
 
-Lemma rel_typ_unsorted_implies_rel_exp {P} {pred_P : PredicativeSig P} : forall {A ρ A' ρ' R},
-    rel_typ_unsorted pred_P A ρ A' ρ' R ->
-    rel_exp A ρ A' ρ' (per_typ pred_P).
+Lemma rel_typ_unsorted_implies_rel_exp {P} {pred_P : PredicativeSig P} : forall {Δ A ρ A' ρ' R},
+    rel_typ_unsorted pred_P Δ A ρ A' ρ' R ->
+    rel_exp Δ A ρ A' ρ' (per_typ pred_P Δ).
 Proof.
   intros.
   destruct_by_head (@rel_typ_unsorted P).
@@ -61,33 +61,33 @@ Proof.
 Qed.
 
 #[export]
-Hint Resolve rel_typ_implies_rel_exp rel_typ_unsorted_implies_rel_exp : mcpts.
+Hint Resolve rel_typ_unsorted_implies_rel_exp : mcpts.
 
-Lemma rel_exp_clean_inversion {P : PtsSig} {pred_P : PredicativeSig P} : forall {Γ env_rel A M M'},
-    {{ EF Γ ≈ Γ ∈ per_ctx_env pred_P ↘ env_rel }} ->
-    {{ ⟪ pred_P ⟫ Γ ⊨ M ≈ M' : A }} ->
-    exists s,
+(* Lemma rel_exp_clean_inversion {P : PtsSig} {pred_P : PredicativeSig P} : forall {Δ Γ env_rel A M M'}, *)
+(*     {{ EF Γ ≈ Γ ∈ per_ctx_env pred_P Δ ↘ env_rel }} -> *)
+(*     {{ ⟪ pred_P ⟫ Δ ▶ Γ ⊨ M ≈ M' : A }} -> *)
+(*     exists s, *)
+(*     forall ρ ρ' (equiv_ρ_ρ' : {{ Dom ρ ≈ ρ' ∈ env_rel }}), *)
+(*     exists (elem_rel : relation (domain P)), *)
+(*       rel_typ pred_P Δ s A ρ A ρ' elem_rel /\ rel_exp M ρ M' ρ' elem_rel. *)
+(* Proof. *)
+(*   intros * ? []. *)
+(*   destruct_conjs. *)
+(*   handle_per_ctx_env_irrel. *)
+(*   eexists. *)
+(*   eassumption. *)
+(* Qed. *)
+
+(* Ltac invert_rel_exp H := *)
+(*   (unshelve (epose proof (rel_exp_clean_inversion _ H); deex); shelve_unifiable; [eassumption |]; clear H) *)
+(*   + dependent destruction H. *)
+
+Lemma rel_exp_unsorted_clean_inversion {P : PtsSig} {pred_P : PredicativeSig P} : forall {Δ Γ env_rel A M M'},
+    {{ EF Γ ≈ Γ ∈ per_ctx_env pred_P Δ ↘ env_rel }} ->
+    {{ ⟪ pred_P ⟫ Δ ▶ Γ ⊨u M ≈ M' : A }} ->
     forall ρ ρ' (equiv_ρ_ρ' : {{ Dom ρ ≈ ρ' ∈ env_rel }}),
     exists (elem_rel : relation (domain P)),
-      rel_typ pred_P s A ρ A ρ' elem_rel /\ rel_exp M ρ M' ρ' elem_rel.
-Proof.
-  intros * ? [].
-  destruct_conjs.
-  handle_per_ctx_env_irrel.
-  eexists.
-  eassumption.
-Qed.
-
-Ltac invert_rel_exp H :=
-  (unshelve (epose proof (rel_exp_clean_inversion _ H); deex); shelve_unifiable; [eassumption |]; clear H)
-  + dependent destruction H.
-
-Lemma rel_exp_unsorted_clean_inversion {P : PtsSig} {pred_P : PredicativeSig P} : forall {Γ env_rel A M M'},
-    {{ EF Γ ≈ Γ ∈ per_ctx_env pred_P ↘ env_rel }} ->
-    {{ ⟪ pred_P ⟫ Γ ⊨u M ≈ M' : A }} ->
-    forall ρ ρ' (equiv_ρ_ρ' : {{ Dom ρ ≈ ρ' ∈ env_rel }}),
-    exists (elem_rel : relation (domain P)),
-      rel_typ_unsorted pred_P A ρ A ρ' elem_rel /\ rel_exp M ρ M' ρ' elem_rel.
+      rel_typ_unsorted pred_P Δ A ρ A ρ' elem_rel /\ rel_exp Δ M ρ M' ρ' elem_rel.
 Proof.
   intros * ? [].
   destruct_conjs.
@@ -106,31 +106,31 @@ Tactic Notation "invert_rel_exp_unsorted" hyp(H) simple_intropattern(l) :=
   invert_rel_exp_unsorted_clean H
   + (destruct H as [l [? H]]; deex_in H).
 
-Lemma rel_exp_implies_rel_exp_unsorted {P} {pred_P : PredicativeSig P} : forall {Γ M M' A},
-    {{ ⟪ pred_P ⟫ Γ ⊨ M ≈ M' : A }} ->
-    {{ ⟪ pred_P ⟫ Γ ⊨u M ≈ M' : A }}.
-Proof.
-  intros.
-  inversion_clear H.
-  destruct_conjs.
-  econstructor; split; mauto.
-  intros.
-  assert (exists elem_rel : relation (domain P),
-             rel_typ pred_P H0 A ρ A ρ' elem_rel /\ rel_exp M ρ M' ρ' elem_rel) by mauto.
-  destruct_conjs.
-  eexists; split; mauto.
-Qed.
+(* Lemma rel_exp_implies_rel_exp_unsorted {P} {pred_P : PredicativeSig P} : forall {Γ M M' A}, *)
+(*     {{ ⟪ pred_P ⟫ Γ ⊨ M ≈ M' : A }} -> *)
+(*     {{ ⟪ pred_P ⟫ Γ ⊨u M ≈ M' : A }}. *)
+(* Proof. *)
+(*   intros. *)
+(*   inversion_clear H. *)
+(*   destruct_conjs. *)
+(*   econstructor; split; mauto. *)
+(*   intros. *)
+(*   assert (exists elem_rel : relation (domain P), *)
+(*              rel_typ pred_P H0 A ρ A ρ' elem_rel /\ rel_exp M ρ M' ρ' elem_rel) by mauto. *)
+(*   destruct_conjs. *)
+(*   eexists; split; mauto. *)
+(* Qed. *)
 
-#[export]
-Hint Resolve rel_exp_implies_rel_exp_unsorted : mcpts.
+(* #[export] *)
+(* Hint Resolve rel_exp_implies_rel_exp_unsorted : mcpts. *)
 
-Lemma rel_sub_clean_inversion1_left {P} {pred_P : PredicativeSig P} : forall {Γ Γ' env_relΓ σ σ' Δ},
-    {{ EF Γ ≈ Γ' ∈ per_ctx_env pred_P ↘ env_relΓ }} ->
-    {{ ⟪ pred_P ⟫ Γ ⊨s σ ≈ σ' : Δ }} ->
-    exists env_relΔ,
-      {{ EF Δ ≈ Δ ∈ per_ctx_env pred_P ↘ env_relΔ }} /\
+Lemma rel_sub_clean_inversion1_left {P} {pred_P : PredicativeSig P} : forall {Δ Γ Γ' Γ'' env_relΓ σ σ'},
+    {{ EF Γ ≈ Γ' ∈ per_ctx_env pred_P Δ ↘ env_relΓ }} ->
+    {{ ⟪ pred_P ⟫ Δ ▶ Γ ⊨s σ ≈ σ' : Γ'' }} ->
+    exists env_relΓ'',
+      {{ EF Γ'' ≈ Γ'' ∈ per_ctx_env pred_P Δ ↘ env_relΓ'' }} /\
         (forall ρ ρ' (equiv_ρ_ρ' : {{ Dom ρ ≈ ρ' ∈ env_relΓ }}),
-            rel_sub σ ρ σ' ρ' env_relΔ).
+            rel_sub Δ σ ρ σ' ρ' env_relΓ'').
 Proof.
   intros * ? [].
   destruct_conjs.
@@ -139,13 +139,13 @@ Proof.
   eassumption.
 Qed.
 
-Lemma rel_sub_clean_inversion1_right {P} {pred_P : PredicativeSig P} : forall {Γ Γ' env_relΓ σ σ' Δ},
-    {{ EF Γ' ≈ Γ ∈ per_ctx_env pred_P ↘ env_relΓ }} ->
-    {{ ⟪ pred_P ⟫ Γ ⊨s σ ≈ σ' : Δ }} ->
-    exists env_relΔ,
-      {{ EF Δ ≈ Δ ∈ per_ctx_env pred_P ↘ env_relΔ }} /\
+Lemma rel_sub_clean_inversion1_right {P} {pred_P : PredicativeSig P} : forall {Δ Γ Γ' Γ'' env_relΓ σ σ'},
+    {{ EF Γ' ≈ Γ ∈ per_ctx_env pred_P Δ ↘ env_relΓ }} ->
+    {{ ⟪ pred_P ⟫ Δ ▶ Γ ⊨s σ ≈ σ' : Γ'' }} ->
+    exists env_relΓ'',
+      {{ EF Γ'' ≈ Γ'' ∈ per_ctx_env pred_P Δ ↘ env_relΓ'' }} /\
         (forall ρ ρ' (equiv_ρ_ρ' : {{ Dom ρ ≈ ρ' ∈ env_relΓ }}),
-            rel_sub σ ρ σ' ρ' env_relΔ).
+            rel_sub Δ σ ρ σ' ρ' env_relΓ'').
 Proof.
   intros * ? [].
   destruct_conjs.
@@ -154,13 +154,13 @@ Proof.
   eassumption.
 Qed.
 
-Lemma rel_sub_clean_inversion2_left {P} {pred_P : PredicativeSig P} : forall {Γ σ σ' Δ Δ' env_relΔ},
-    {{ EF Δ ≈ Δ' ∈ per_ctx_env pred_P ↘ env_relΔ }} ->
-    {{ ⟪ pred_P ⟫  Γ ⊨s σ ≈ σ' : Δ }} ->
+Lemma rel_sub_clean_inversion2_left {P} {pred_P : PredicativeSig P} : forall {Δ Γ σ σ' Γ' Γ'' env_relΓ'},
+    {{ EF Γ' ≈ Γ'' ∈ per_ctx_env pred_P Δ ↘ env_relΓ' }} ->
+    {{ ⟪ pred_P ⟫ Δ ▶ Γ ⊨s σ ≈ σ' : Γ' }} ->
     exists env_relΓ,
-      {{ EF Γ ≈ Γ ∈ per_ctx_env pred_P ↘ env_relΓ }} /\
+      {{ EF Γ ≈ Γ ∈ per_ctx_env pred_P Δ ↘ env_relΓ }} /\
         (forall ρ ρ' (equiv_ρ_ρ' : {{ Dom ρ ≈ ρ' ∈ env_relΓ }}),
-            rel_sub σ ρ σ' ρ' env_relΔ).
+            rel_sub Δ σ ρ σ' ρ' env_relΓ').
 Proof.
   intros * ? [].
   destruct_conjs.
@@ -169,13 +169,13 @@ Proof.
   eassumption.
 Qed.
 
-Lemma rel_sub_clean_inversion2_right {P} {pred_P : PredicativeSig P} : forall {Γ σ σ' Δ Δ' env_relΔ},
-    {{ EF Δ' ≈ Δ ∈ per_ctx_env pred_P ↘ env_relΔ }} ->
-    {{ ⟪ pred_P ⟫ Γ ⊨s σ ≈ σ' : Δ }} ->
+Lemma rel_sub_clean_inversion2_right {P} {pred_P : PredicativeSig P} : forall {Δ Γ σ σ' Γ' Γ'' env_relΓ'},
+    {{ EF Γ'' ≈ Γ' ∈ per_ctx_env pred_P Δ ↘ env_relΓ' }} ->
+    {{ ⟪ pred_P ⟫ Δ ▶ Γ ⊨s σ ≈ σ' : Γ' }} ->
     exists env_relΓ,
-      {{ EF Γ ≈ Γ ∈ per_ctx_env pred_P ↘ env_relΓ }} /\
+      {{ EF Γ ≈ Γ ∈ per_ctx_env pred_P Δ ↘ env_relΓ }} /\
         (forall ρ ρ' (equiv_ρ_ρ' : {{ Dom ρ ≈ ρ' ∈ env_relΓ }}),
-            rel_sub σ ρ σ' ρ' env_relΔ).
+            rel_sub Δ σ ρ σ' ρ' env_relΓ').
 Proof.
   intros * ? [].
   destruct_conjs.
@@ -184,12 +184,12 @@ Proof.
   eassumption.
 Qed.
 
-Lemma rel_sub_clean_inversion3_left_left {P} {pred_P : PredicativeSig P} : forall {Γ Γ' env_relΓ σ σ' Δ Δ' env_relΔ},
-    {{ EF Γ ≈ Γ' ∈ per_ctx_env pred_P ↘ env_relΓ }} ->
-    {{ EF Δ ≈ Δ' ∈ per_ctx_env pred_P ↘ env_relΔ }} ->
-    {{ ⟪ pred_P ⟫ Γ ⊨s σ ≈ σ' : Δ }} ->
-    forall ρ ρ' (equiv_ρ_ρ' : {{ Dom ρ ≈ ρ' ∈ env_relΓ }}),
-      rel_sub σ ρ σ' ρ' env_relΔ.
+Lemma rel_sub_clean_inversion3_left_left {P} {pred_P : PredicativeSig P} : forall {Δ Γ1 Γ1' env_relΓ1 σ σ' Γ2 Γ2' env_relΓ2},
+    {{ EF Γ1 ≈ Γ1' ∈ per_ctx_env pred_P Δ ↘ env_relΓ1 }} ->
+    {{ EF Γ2 ≈ Γ2' ∈ per_ctx_env pred_P Δ ↘ env_relΓ2 }} ->
+    {{ ⟪ pred_P ⟫ Δ ▶ Γ1 ⊨s σ ≈ σ' : Γ2 }} ->
+    forall ρ ρ' (equiv_ρ_ρ' : {{ Dom ρ ≈ ρ' ∈ env_relΓ1 }}),
+      rel_sub Δ σ ρ σ' ρ' env_relΓ2.
 Proof.
   intros * HΓ ?.
   intros []%(rel_sub_clean_inversion1_left HΓ).
@@ -198,12 +198,12 @@ Proof.
   eassumption.
 Qed.
 
-Lemma rel_sub_clean_inversion3_left_right {P} {pred_P : PredicativeSig P} : forall {Γ Γ' env_relΓ σ σ' Δ Δ' env_relΔ},
-    {{ EF Γ ≈ Γ' ∈ per_ctx_env pred_P ↘ env_relΓ }} ->
-    {{ EF Δ' ≈ Δ ∈ per_ctx_env pred_P ↘ env_relΔ }} ->
-    {{ ⟪ pred_P ⟫ Γ ⊨s σ ≈ σ' : Δ }} ->
-    forall ρ ρ' (equiv_ρ_ρ' : {{ Dom ρ ≈ ρ' ∈ env_relΓ }}),
-      rel_sub σ ρ σ' ρ' env_relΔ.
+Lemma rel_sub_clean_inversion3_left_right {P} {pred_P : PredicativeSig P} : forall {Δ Γ1 Γ1' env_relΓ1 σ σ' Γ2 Γ2' env_relΓ2},
+    {{ EF Γ1 ≈ Γ1' ∈ per_ctx_env pred_P Δ ↘ env_relΓ1 }} ->
+    {{ EF Γ2' ≈ Γ2 ∈ per_ctx_env pred_P Δ ↘ env_relΓ2 }} ->
+    {{ ⟪ pred_P ⟫ Δ ▶ Γ1 ⊨s σ ≈ σ' : Γ2 }} ->
+    forall ρ ρ' (equiv_ρ_ρ' : {{ Dom ρ ≈ ρ' ∈ env_relΓ1 }}),
+      rel_sub Δ σ ρ σ' ρ' env_relΓ2.
 Proof.
   intros * HΓ ?.
   intros []%(rel_sub_clean_inversion1_left HΓ).
@@ -212,12 +212,12 @@ Proof.
   eassumption.
 Qed.
 
-Lemma rel_sub_clean_inversion3_right_left {P} {pred_P : PredicativeSig P}  : forall {Γ Γ' env_relΓ σ σ' Δ Δ' env_relΔ},
-    {{ EF Γ' ≈ Γ ∈ per_ctx_env pred_P ↘ env_relΓ }} ->
-    {{ EF Δ ≈ Δ' ∈ per_ctx_env pred_P ↘ env_relΔ }} ->
-    {{ ⟪ pred_P ⟫ Γ ⊨s σ ≈ σ' : Δ }} ->
-    forall ρ ρ' (equiv_ρ_ρ' : {{ Dom ρ ≈ ρ' ∈ env_relΓ }}),
-      rel_sub σ ρ σ' ρ' env_relΔ.
+Lemma rel_sub_clean_inversion3_right_left {P} {pred_P : PredicativeSig P}  : forall {Δ Γ1 Γ1' env_relΓ1 σ σ' Γ2 Γ2' env_relΓ2},
+    {{ EF Γ1' ≈ Γ1 ∈ per_ctx_env pred_P Δ ↘ env_relΓ1 }} ->
+    {{ EF Γ2 ≈ Γ2' ∈ per_ctx_env pred_P Δ ↘ env_relΓ2 }} ->
+    {{ ⟪ pred_P ⟫ Δ ▶ Γ1 ⊨s σ ≈ σ' : Γ2 }} ->
+    forall ρ ρ' (equiv_ρ_ρ' : {{ Dom ρ ≈ ρ' ∈ env_relΓ1 }}),
+      rel_sub Δ σ ρ σ' ρ' env_relΓ2.
 Proof.
   intros * HΓ ?.
   intros []%(rel_sub_clean_inversion1_right HΓ).
@@ -226,12 +226,12 @@ Proof.
   eassumption.
 Qed.
 
-Lemma rel_sub_clean_inversion3_right_right {P} {pred_P : PredicativeSig P} : forall {Γ Γ' env_relΓ σ σ' Δ Δ' env_relΔ},
-    {{ EF Γ' ≈ Γ ∈ per_ctx_env pred_P ↘ env_relΓ }} ->
-    {{ EF Δ' ≈ Δ ∈ per_ctx_env pred_P ↘ env_relΔ }} ->
-    {{ ⟪ pred_P ⟫ Γ ⊨s σ ≈ σ' : Δ }} ->
-    forall ρ ρ' (equiv_ρ_ρ' : {{ Dom ρ ≈ ρ' ∈ env_relΓ }}),
-      rel_sub σ ρ σ' ρ' env_relΔ.
+Lemma rel_sub_clean_inversion3_right_right {P} {pred_P : PredicativeSig P} : forall {Δ Γ1 Γ1' env_relΓ1 σ σ' Γ2 Γ2' env_relΓ2},
+    {{ EF Γ1' ≈ Γ1 ∈ per_ctx_env pred_P Δ ↘ env_relΓ1 }} ->
+    {{ EF Γ2' ≈ Γ2 ∈ per_ctx_env pred_P Δ ↘ env_relΓ2 }} ->
+    {{ ⟪ pred_P ⟫ Δ ▶ Γ1 ⊨s σ ≈ σ' : Γ2 }} ->
+    forall ρ ρ' (equiv_ρ_ρ' : {{ Dom ρ ≈ ρ' ∈ env_relΓ1 }}),
+      rel_sub Δ σ ρ σ' ρ' env_relΓ2.
 Proof.
   intros * HΓ ?.
   intros []%(rel_sub_clean_inversion1_right HΓ).
