theories/Core/Completeness/TermStructureCases.v
@@ -6,14 +6,14 @@ From McPTS.Core.Completeness Require Import LogicalRelation SortCases.
 Import Domain_Notations.
 
 
-Lemma rel_exp_sub_cong {P : PtsSig} {pred_P : PredicativeSig P} : forall {Δ M M' A σ σ' Γ},
-    {{ ⟪ pred_P ⟫ Δ ⊨u M ≈ M' : A }} ->
-    {{ ⟪ pred_P ⟫ Γ ⊨s σ ≈ σ' : Δ }} ->
-    {{ ⟪ pred_P ⟫ Γ ⊨u M[σ] ≈ M'[σ'] : A[σ] }}.
+Lemma rel_exp_sub_cong {P : PtsSig} {pred_P : PredicativeSig P} : forall {Δ Γ Γ' M M' A σ σ'},
+    {{ ⟪ pred_P ⟫ Δ ▶ Γ' ⊨u M ≈ M' : A }} ->
+    {{ ⟪ pred_P ⟫ Δ ▶ Γ ⊨s σ ≈ σ' : Γ' }} ->
+    {{ ⟪ pred_P ⟫ Δ ▶ Γ ⊨u M[σ] ≈ M'[σ'] : A[σ] }}.
 Proof with mautosolve.
-  intros * [env_relΔ] [env_relΓ].
+  intros * [env_relΓ'] [env_relΓ].
   destruct_conjs.
-  pose env_relΔ.
+  pose env_relΓ'.
   handle_per_ctx_env_irrel.
   eexists; split; [eassumption |].
   intros.
@@ -22,13 +22,13 @@ Proof with mautosolve.
   (on_all_hyp: destruct_rel_by_assumption env_relΓ).
   handle_per_typ_elem_irrel.
   match goal with
-  | _: {{ ⟦ σ ⟧s ρ ↘ ^?ρ0 }},
-      _: {{ ⟦ σ ⟧s ρ' ↘ ^?ρ'0 }} |- _ =>
+  | _: {{ Δ ▶  ⟦ σ ⟧s ρ ↘ ^?ρ0 }},
+      _: {{ Δ ▶  ⟦ σ ⟧s ρ' ↘ ^?ρ'0 }} |- _ =>
       rename ρ0 into ρσ;
       rename ρ'0 into ρ'σ
   end.
-  assert (env_relΔ ρσ ρ'σ) by (etransitivity; [|symmetry; eassumption]; eassumption).
-  (on_all_hyp: destruct_rel_by_assumption env_relΔ).
+  assert (env_relΓ' ρσ ρ'σ) by (etransitivity; [|symmetry; eassumption]; eassumption).
+  (on_all_hyp: destruct_rel_by_assumption env_relΓ').
   destruct_by_head (@rel_typ_unsorted P).
   destruct_by_head (@rel_exp P).
   handle_per_typ_elem_irrel.
@@ -40,9 +40,9 @@ Qed.
 #[export]
 Hint Resolve rel_exp_sub_cong : mcpts.
 
-Lemma rel_exp_sub_sort_rel_exp_no_sub {P} {pred_P : PredicativeSig P} : forall {Γ A B σ s},
-    {{ ⟪ pred_P ⟫ Γ ⊨u A ≈ B : Sort@s[σ] }} ->
-    {{ ⟪ pred_P ⟫ Γ ⊨u A ≈ B : Sort@s }}.
+Lemma rel_exp_sub_sort_rel_exp_no_sub {P} {pred_P : PredicativeSig P} : forall {Δ Γ A B σ s},
+    {{ ⟪ pred_P ⟫ Δ ▶ Γ ⊨u A ≈ B : Sort@s[σ] }} ->
+    {{ ⟪ pred_P ⟫ Δ ▶ Γ ⊨u A ≈ B : Sort@s }}.
 Proof.
   intros * [relΓ []].
   eexists; split; mauto 2.
@@ -50,7 +50,7 @@ Proof.
   specialize (H0 ρ ρ' equiv_ρ_ρ') as [elem_rel []].
   destruct H0.
   simplify_evals.
-  assert (per_typ_elem pred_P (per_sort pred_P s) d{{{ Sort@s }}} d{{{ Sort@s }}}) by (econstructor; reflexivity).
+  assert (per_typ_elem pred_P Δ (per_sort pred_P Δ s) d{{{ Sort@s }}} d{{{ Sort@s }}}) by (econstructor; reflexivity).
   handle_per_typ_elem_irrel.
   eexists; split; mauto 2.
   econstructor; mauto 2.
@@ -59,22 +59,22 @@ Qed.
 #[local]
 Hint Resolve rel_exp_sub_sort_rel_exp_no_sub : mcpts.
 
-Lemma rel_exp_sub_cong_sort {P} {pred_P : PredicativeSig P} : forall {Δ A A' s σ σ' Γ},
-    {{ ⟪ pred_P ⟫ Δ ⊨u A ≈ A' : Sort@s }} ->
-    {{ ⟪ pred_P ⟫ Γ ⊨s σ ≈ σ' : Δ }} ->
-    {{ ⟪ pred_P ⟫ Γ ⊨u A[σ] ≈ A'[σ'] : Sort@s }}.
+Lemma rel_exp_sub_cong_sort {P} {pred_P : PredicativeSig P} : forall {Δ Γ Γ' A A' s σ σ'},
+    {{ ⟪ pred_P ⟫ Δ ▶ Γ' ⊨u A ≈ A' : Sort@s }} ->
+    {{ ⟪ pred_P ⟫ Δ ▶ Γ ⊨s σ ≈ σ' : Γ' }} ->
+    {{ ⟪ pred_P ⟫ Δ ▶ Γ ⊨u A[σ] ≈ A'[σ'] : Sort@s }}.
 Proof with mautosolve.
   intros.
-  assert {{ ⟪ pred_P ⟫ Γ ⊨u A[σ] ≈ A'[σ'] : Sort@s[σ] }} by mauto 2.
+  assert {{ ⟪ pred_P ⟫ Δ ▶ Γ ⊨u A[σ] ≈ A'[σ'] : Sort@s[σ] }} by mauto 2.
   mauto 2.
 Qed.
 
 #[export]
 Hint Resolve rel_exp_sub_cong_sort : mcpts.
 
-Lemma rel_exp_sub_id {P : PtsSig} {pred_P : PredicativeSig P} : forall {Γ M A},
-    {{ ⟪ pred_P ⟫ Γ ⊨u M : A }} ->
-    {{ ⟪ pred_P ⟫ Γ ⊨u M[Id] ≈ M : A }}.
+Lemma rel_exp_sub_id {P : PtsSig} {pred_P : PredicativeSig P} : forall {Δ Γ M A},
+    {{ ⟪ pred_P ⟫ Δ ▶ Γ ⊨u M : A }} ->
+    {{ ⟪ pred_P ⟫ Δ ▶ Γ ⊨u M[Id] ≈ M : A }}.
 Proof with mautosolve.
   intros * [env_relΓ].
   destruct_conjs.
@@ -90,11 +90,11 @@ Qed.
 #[export]
 Hint Resolve rel_exp_sub_id : mcpts.
 
-Lemma rel_exp_sub_compose {P : PtsSig} {pred_P : PredicativeSig P} : forall {Γ τ Γ' σ Γ'' M A},
-    {{ ⟪ pred_P ⟫ Γ ⊨s τ : Γ' }} ->
-    {{ ⟪ pred_P ⟫ Γ' ⊨s σ : Γ'' }} ->
-    {{ ⟪ pred_P ⟫ Γ'' ⊨u M : A }} ->
-    {{ ⟪ pred_P ⟫ Γ ⊨u M[σ ∘ τ] ≈ M[σ][τ] : A[σ ∘ τ] }}.
+Lemma rel_exp_sub_compose {P : PtsSig} {pred_P : PredicativeSig P} : forall {Δ Γ τ Γ' σ Γ'' M A},
+    {{ ⟪ pred_P ⟫ Δ ▶ Γ ⊨s τ : Γ' }} ->
+    {{ ⟪ pred_P ⟫ Δ ▶ Γ' ⊨s σ : Γ'' }} ->
+    {{ ⟪ pred_P ⟫ Δ ▶ Γ'' ⊨u M : A }} ->
+    {{ ⟪ pred_P ⟫ Δ ▶ Γ ⊨u M[σ ∘ τ] ≈ M[σ][τ] : A[σ ∘ τ] }}.
 Proof with mautosolve.
   intros * [env_relΓ [? [env_relΓ']]] [? [? [env_relΓ'']]] HM.
   destruct_conjs.
@@ -120,14 +120,14 @@ Qed.
 #[export]
 Hint Resolve rel_exp_sub_compose : mcpts.
 
-Lemma rel_exp_sub_compose_sort {P : PtsSig} {pred_P : PredicativeSig P} : forall {Γ τ Γ' σ Γ'' A s},
-    {{ ⟪ pred_P ⟫ Γ ⊨s τ : Γ' }} ->
-    {{ ⟪ pred_P ⟫ Γ' ⊨s σ : Γ'' }} ->
-    {{ ⟪ pred_P ⟫ Γ'' ⊨u A : Sort@s }} ->
-    {{ ⟪ pred_P ⟫ Γ ⊨u A[σ∘τ] ≈ A[σ][τ] : Sort@s }}.
+Lemma rel_exp_sub_compose_sort {P : PtsSig} {pred_P : PredicativeSig P} : forall {Δ Γ τ Γ' σ Γ'' A s},
+    {{ ⟪ pred_P ⟫ Δ ▶ Γ ⊨s τ : Γ' }} ->
+    {{ ⟪ pred_P ⟫ Δ ▶ Γ' ⊨s σ : Γ'' }} ->
+    {{ ⟪ pred_P ⟫ Δ ▶ Γ'' ⊨u A : Sort@s }} ->
+    {{ ⟪ pred_P ⟫ Δ ▶ Γ ⊨u A[σ∘τ] ≈ A[σ][τ] : Sort@s }}.
 Proof with mautosolve.
   intros.
-  assert {{ ⟪ pred_P ⟫ Γ ⊨u A[σ∘τ] ≈ A[σ][τ] : Sort@s[σ∘τ] }} by mauto 2.
+  assert {{ ⟪ pred_P ⟫ Δ ▶ Γ ⊨u A[σ∘τ] ≈ A[σ][τ] : Sort@s[σ∘τ] }} by mauto 2.
   mauto 2.
 Qed.
 
@@ -135,10 +135,10 @@ Qed.
 Hint Resolve rel_exp_sub_compose_sort : mcpts.
 
 
-Lemma rel_exp_conv_typ {P : PtsSig} {pred_P : PredicativeSig P} : forall {Γ M M' A A'},
-    {{ ⟪ pred_P ⟫ Γ ⊨u M ≈ M' : A }} ->
-    {{ ⟪ pred_P ⟫ Γ ⊨ A ≈ A' }} ->
-    {{ ⟪ pred_P ⟫ Γ ⊨u M ≈ M' : A' }}.
+Lemma rel_exp_conv_typ {P : PtsSig} {pred_P : PredicativeSig P} : forall {Δ Γ M M' A A'},
+    {{ ⟪ pred_P ⟫ Δ ▶ Γ ⊨u M ≈ M' : A }} ->
+    {{ ⟪ pred_P ⟫ Δ ▶ Γ ⊨ A ≈ A' }} ->
+    {{ ⟪ pred_P ⟫ Δ ▶ Γ ⊨u M ≈ M' : A' }}.
 Proof with mautosolve.
   intros.
   invert_rel_exp_unsorted H;
@@ -156,9 +156,9 @@ Proof with mautosolve.
   assert (equiv_ρ'_ρ : env_relΓ ρ' ρ) by (symmetry; mauto).
   assert (equiv_ρ'_ρ' : env_relΓ ρ' ρ') by (etransitivity; [|symmetry]; eassumption).
 
-  assert (exists elem_rel : relation (domain P), rel_typ_unsorted pred_P A ρ A ρ' elem_rel /\ rel_exp M ρ M' ρ' elem_rel) by mauto.
-  assert (exists elem_rel : relation (domain P), rel_typ_unsorted pred_P A ρ' A' ρ' elem_rel) by mauto.
-  assert (exists elem_rel : relation (domain P), rel_typ_unsorted pred_P A ρ A' ρ elem_rel) by mauto.
+  assert (exists elem_rel : relation (domain P), rel_typ_unsorted pred_P Δ A ρ A ρ' elem_rel /\ rel_exp Δ M ρ M' ρ' elem_rel) by mauto.
+  assert (exists elem_rel : relation (domain P), rel_typ_unsorted pred_P Δ A ρ' A' ρ' elem_rel) by mauto.
+  assert (exists elem_rel : relation (domain P), rel_typ_unsorted pred_P Δ A ρ A' ρ elem_rel) by mauto.
   destruct_conjs.
   eexists; split; mauto 2.
 
@@ -170,9 +170,9 @@ Proof with mautosolve.
   transitivity a'1; mauto.
 Qed.
 
-Lemma rel_typ_implies_rel_typ_unsorted {P} {pred_P : PredicativeSig P} : forall {Γ A A' s},
-    {{ ⟪ pred_P ⟫ Γ ⊨u A ≈ A' : Sort@s }} ->
-    {{ ⟪ pred_P ⟫ Γ ⊨ A ≈ A' }}.
+Lemma rel_typ_implies_rel_typ_unsorted {P} {pred_P : PredicativeSig P} : forall {Δ Γ A A' s},
+    {{ ⟪ pred_P ⟫ Δ ▶ Γ ⊨u A ≈ A' : Sort@s }} ->
+    {{ ⟪ pred_P ⟫ Δ ▶ Γ ⊨ A ≈ A' }}.
 Proof.
   intros * [relΓ []].
   eexists; split; mauto 2.
@@ -181,30 +181,30 @@ Proof.
   destruct H1.
   destruct H0.
   simplify_evals.
-  assert (per_typ_elem pred_P (per_sort pred_P s) d{{{ Sort@s }}} d{{{ Sort@s }}}) by (eapply per_typ_sort; reflexivity).
+  assert (per_typ_elem pred_P Δ (per_sort pred_P Δ s) d{{{ Sort@s }}} d{{{ Sort@s }}}) by (eapply per_typ_sort; reflexivity).
   handle_per_typ_elem_irrel.
   destruct H3 as [].
-  assert (per_typ_elem pred_P x m m') by mauto 3.
+  assert (per_typ_elem pred_P Δ x m m') by mauto 3.
   eexists.
   econstructor; mauto 2.
 Qed.
 
-Lemma rel_exp_conv {P : PtsSig} {pred_P : PredicativeSig P} : forall {Γ M M' A A' s},
-    {{ ⟪ pred_P ⟫ Γ ⊨u M ≈ M' : A }} ->
-    {{ ⟪ pred_P ⟫ Γ ⊨u A ≈ A' : Sort@s }} ->
-    {{ ⟪ pred_P ⟫ Γ ⊨u M ≈ M' : A' }}.
+Lemma rel_exp_conv {P : PtsSig} {pred_P : PredicativeSig P} : forall {Δ Γ M M' A A' s},
+    {{ ⟪ pred_P ⟫ Δ ▶ Γ ⊨u M ≈ M' : A }} ->
+    {{ ⟪ pred_P ⟫ Δ ▶ Γ ⊨u A ≈ A' : Sort@s }} ->
+    {{ ⟪ pred_P ⟫ Δ ▶ Γ ⊨u M ≈ M' : A' }}.
 Proof with mautosolve.
   intros.
-  assert {{ ⟪ pred_P ⟫ Γ ⊨ A ≈ A' }} by (eapply rel_typ_implies_rel_typ_unsorted; mauto 2).
+  assert {{ ⟪ pred_P ⟫ Δ ▶ Γ ⊨ A ≈ A' }} by (eapply rel_typ_implies_rel_typ_unsorted; mauto 2).
   eapply rel_exp_conv_typ; mauto 2.
 Qed.
 
 #[export]
 Hint Resolve rel_exp_conv : mcpts.
 
-Lemma rel_exp_sym {P : PtsSig} {pred_P : PredicativeSig P} : forall {Γ M M' A},
-    {{ ⟪ pred_P ⟫ Γ ⊨u M ≈ M' : A }} ->
-    {{ ⟪ pred_P ⟫ Γ ⊨u M' ≈ M : A }}.
+Lemma rel_exp_sym {P : PtsSig} {pred_P : PredicativeSig P} : forall {Δ Γ M M' A},
+    {{ ⟪ pred_P ⟫ Δ ▶ Γ ⊨u M ≈ M' : A }} ->
+    {{ ⟪ pred_P ⟫ Δ ▶ Γ ⊨u M' ≈ M : A }}.
 Proof with mautosolve.
   intros * [env_relΓ].
   destruct_conjs.
@@ -224,10 +224,10 @@ Qed.
 #[export]
 Hint Resolve rel_exp_sym : mcpts.
 
-Lemma rel_exp_trans {P : PtsSig} {pred_P : PredicativeSig P} : forall {Γ M1 M2 M3 A},
-    {{ ⟪ pred_P ⟫ Γ ⊨u M1 ≈ M2 : A }} ->
-    {{ ⟪ pred_P ⟫ Γ ⊨u M2 ≈ M3 : A }} ->
-    {{ ⟪ pred_P ⟫ Γ ⊨u M1 ≈ M3 : A }}.
+Lemma rel_exp_trans {P : PtsSig} {pred_P : PredicativeSig P} : forall {Δ Γ M1 M2 M3 A},
+    {{ ⟪ pred_P ⟫ Δ ▶ Γ ⊨u M1 ≈ M2 : A }} ->
+    {{ ⟪ pred_P ⟫ Δ ▶ Γ ⊨u M2 ≈ M3 : A }} ->
+    {{ ⟪ pred_P ⟫ Δ ▶ Γ ⊨u M1 ≈ M3 : A }}.
 Proof with mautosolve.
   intros * [env_relΓ] HM2M3.
   destruct_conjs.
@@ -249,14 +249,14 @@ Qed.
 Hint Resolve rel_exp_trans : mcpts.
 
 #[export]
-Instance rel_exp_unsorted_PER {P : PtsSig} {pred_P : PredicativeSig P} {Γ A} : PER (rel_exp_under_ctx_unsorted pred_P Γ A).
+Instance rel_exp_unsorted_PER {P : PtsSig} {pred_P : PredicativeSig P} {Δ Γ A} : PER (rel_exp_under_ctx_unsorted pred_P Δ Γ A).
 Proof.
   split; mauto.
 Qed.
 
-Lemma rel_typ_sort_refl {P} {pred_P : PredicativeSig P} : forall {Γ s},
-    {{ ⟪ pred_P ⟫ ⊨ Γ }} ->
-    {{ ⟪ pred_P ⟫ Γ ⊨ Sort@s ≈ Sort@s }}.
+Lemma rel_typ_sort_refl {P} {pred_P : PredicativeSig P} : forall {Δ Γ s},
+    {{ ⟪ pred_P ⟫ Δ ▶ Γ }} ->
+    {{ ⟪ pred_P ⟫ Δ ▶ Γ ⊨ Sort@s ≈ Sort@s }}.
 Proof.
   intros * [env_relΓ].
   eexists; split; [eassumption|].
@@ -266,38 +266,43 @@ Proof.
 Qed.
 
 
-Lemma rel_typ_of_rel_sort {P} {pred_P : PredicativeSig P} : forall {Γ A A' s},
-    {{ ⟪ pred_P ⟫ Γ ⊨u A ≈ A' : Sort@s }} ->
-    {{ ⟪ pred_P ⟫ Γ ⊨ A ≈ A' }}.
+Lemma rel_typ_of_rel_sort {P} {pred_P : PredicativeSig P} : forall {Δ Γ A A' s},
+    {{ ⟪ pred_P ⟫ Δ ▶ Γ ⊨u A ≈ A' : Sort@s }} ->
+    {{ ⟪ pred_P ⟫ Δ ▶ Γ ⊨ A ≈ A' }}.
 Proof.
   intros * [env_relΓ].
   destruct_conjs.
   eexists; split; [eassumption|].
   intros.
   assert (exists elem_rel : relation (domain P),
-      rel_typ_unsorted pred_P {{{ Sort@s }}} ρ {{{ Sort@s }}} ρ' elem_rel /\
-      rel_exp A ρ A' ρ' elem_rel) by mauto.
+      rel_typ_unsorted pred_P Δ {{{ Sort@s }}} ρ {{{ Sort@s }}} ρ' elem_rel /\
+      rel_exp Δ A ρ A' ρ' elem_rel) by mauto.
   destruct_conjs.
 
 
   destruct_by_head (@rel_typ_unsorted P).
-  assert (per_typ_elem pred_P (per_sort pred_P s) a a').
+  assert (per_typ_elem pred_P Δ (per_sort pred_P Δ s) a a').
   {
     inversion H2; inversion H4; subst.
     econstructor; reflexivity.
   }
   handle_per_typ_elem_irrel.
-  assert (exists R, rel_typ pred_P s A ρ A' ρ' R) by mauto.
-  destruct_conjs.
-  eexists; mauto.
+  specialize (H0 _ _ equiv_ρ_ρ') as [elem_rel []].
+  destruct_by_head (@rel_exp).
+  destruct_rel_typ_unsorted.
+  simplify_evals.
+  handle_per_typ_elem_irrel.
+  destruct H11.
+  assert (per_typ_elem pred_P Δ x m0 m'0) by mauto 3.
+  eexists; mauto.  
 Qed.
 
 #[export]
 Hint Resolve rel_typ_of_rel_sort : mcpts.
 
-Lemma val_typ_of_val_sort {P} {pred_P : PredicativeSig P} : forall {Γ A s},
-    {{ ⟪ pred_P ⟫ Γ ⊨u A : Sort@s }} ->
-    {{ ⟪ pred_P ⟫ Γ ⊨ A }}.
+Lemma val_typ_of_val_sort {P} {pred_P : PredicativeSig P} : forall {Δ Γ A s},
+    {{ ⟪ pred_P ⟫ Δ ▶ Γ ⊨u A : Sort@s }} ->
+    {{ ⟪ pred_P ⟫ Δ ▶ Γ ⊨ A }}.
 Proof.
   intros * HA.
   eapply rel_typ_of_rel_sort; mauto.
@@ -306,10 +311,10 @@ Qed.
 #[export]
 Hint Resolve val_typ_of_val_sort : mcpts.
 
-Lemma rel_typ_sub_cong {P} {pred_P : PredicativeSig P} : forall {Γ Δ σ σ' A A'},
-      {{ ⟪ pred_P ⟫ Γ ⊨s σ ≈ σ' : Δ }} ->
-      {{ ⟪ pred_P ⟫ Δ ⊨ A ≈ A' }} ->
-      {{ ⟪ pred_P ⟫ Γ ⊨ A[σ] ≈ A'[σ'] }}.
+Lemma rel_typ_sub_cong {P} {pred_P : PredicativeSig P} : forall {Δ Γ Γ' σ σ' A A'},
+      {{ ⟪ pred_P ⟫ Δ ▶ Γ ⊨s σ ≈ σ' : Γ' }} ->
+      {{ ⟪ pred_P ⟫ Δ ▶ Γ' ⊨ A ≈ A' }} ->
+      {{ ⟪ pred_P ⟫ Δ ▶ Γ ⊨ A[σ] ≈ A'[σ'] }}.
 Proof.
   intros * [env_relΓ [? [env_relΔ]]] [?].
   destruct_conjs.
@@ -317,9 +322,9 @@ Proof.
   eexists; split; [eassumption|].
   intros.
 
-  assert (rel_sub σ ρ σ' ρ' env_relΔ) by mauto.
+  assert (rel_sub Δ σ ρ σ' ρ' env_relΔ) by mauto.
   destruct_by_head (@rel_sub P).
-  assert (exists elem_rel : relation (domain P), rel_typ_unsorted pred_P A ρσ A' ρ'σ' elem_rel) by mauto.
+  assert (exists elem_rel : relation (domain P), rel_typ_unsorted pred_P Δ A ρσ A' ρ'σ' elem_rel) by mauto.
   destruct_conjs.
   destruct_by_head (@rel_typ_unsorted P).
   eexists; econstructor; mauto.
@@ -328,10 +333,10 @@ Qed.
 #[export]
 Hint Resolve rel_typ_sub_cong : mcpts.
 
-Lemma val_typ_sub {P} {pred_P : PredicativeSig P} : forall {Γ Δ σ A},
-    {{ ⟪ pred_P ⟫ Γ ⊨s σ : Δ }} ->
-    {{ ⟪ pred_P ⟫ Δ ⊨ A }} ->
-    {{ ⟪ pred_P ⟫ Γ ⊨ A[σ] }}.
+Lemma val_typ_sub {P} {pred_P : PredicativeSig P} : forall {Δ Γ Γ' σ A},
+    {{ ⟪ pred_P ⟫ Δ ▶ Γ ⊨s σ : Γ' }} ->
+    {{ ⟪ pred_P ⟫ Δ ▶ Γ' ⊨ A }} ->
+    {{ ⟪ pred_P ⟫ Δ ▶ Γ ⊨ A[σ] }}.
 Proof.
   intros * Hσ HA.
   eapply rel_typ_sub_cong; mauto.
@@ -340,11 +345,11 @@ Qed.
 #[export]
 Hint Resolve val_typ_sub : mcpts.
 
-Lemma rel_typ_sub_compose {P} {pred_P : PredicativeSig P} : forall {Γ τ Γ' σ Γ'' A},
-    {{ ⟪ pred_P ⟫ Γ ⊨s τ : Γ' }} ->
-    {{ ⟪ pred_P ⟫ Γ' ⊨s σ : Γ'' }} ->
-    {{ ⟪ pred_P ⟫ Γ'' ⊨ A }} ->
-    {{ ⟪ pred_P ⟫ Γ ⊨ A[σ ∘ τ] ≈ A[σ][τ] }}.
+Lemma rel_typ_sub_compose {P} {pred_P : PredicativeSig P} : forall {Δ Γ τ Γ' σ Γ'' A},
+    {{ ⟪ pred_P ⟫ Δ ▶ Γ ⊨s τ : Γ' }} ->
+    {{ ⟪ pred_P ⟫ Δ ▶ Γ' ⊨s σ : Γ'' }} ->
+    {{ ⟪ pred_P ⟫ Δ ▶ Γ'' ⊨ A }} ->
+    {{ ⟪ pred_P ⟫ Δ ▶ Γ ⊨ A[σ ∘ τ] ≈ A[σ][τ] }}.
 Proof.
   intros * [env_relΓ [? [env_relΓ']]] [? [? [env_relΓ'']]] HA.
   destruct HA.
@@ -353,11 +358,11 @@ Proof.
   eexists; split; [eassumption |].
 
   intros.
-  assert (rel_sub τ ρ τ ρ' env_relΓ') by mauto.
+  assert (rel_sub Δ τ ρ τ ρ' env_relΓ') by mauto.
   destruct_by_head (@rel_sub P).
-  assert (rel_sub σ ρσ σ ρ'σ' env_relΓ'') by mauto.
+  assert (rel_sub Δ σ ρσ σ ρ'σ' env_relΓ'') by mauto.
   destruct_by_head (@rel_sub P).
-  assert (exists elem_rel : relation (domain P), rel_typ_unsorted pred_P A ρσ0 A ρ'σ'0 elem_rel) by mauto.
+  assert (exists elem_rel : relation (domain P), rel_typ_unsorted pred_P Δ A ρσ0 A ρ'σ'0 elem_rel) by mauto.
   destruct_conjs.
   destruct_by_head (@rel_typ_unsorted P).
 
@@ -368,15 +373,15 @@ Qed.
 #[export]
 Hint Resolve rel_typ_sub_compose : mcpts.
 
-Lemma rel_typ_sub_id {P} {pred_P : PredicativeSig P} : forall {Γ A},
-    {{ ⟪ pred_P ⟫ Γ ⊨ A }} ->
-    {{ ⟪ pred_P ⟫ Γ ⊨ A[Id] ≈ A }}.
+Lemma rel_typ_sub_id {P} {pred_P : PredicativeSig P} : forall {Δ Γ A},
+    {{ ⟪ pred_P ⟫ Δ ▶ Γ ⊨ A }} ->
+    {{ ⟪ pred_P ⟫ Δ ▶ Γ ⊨ A[Id] ≈ A }}.
 Proof.
   intros * [env_relΓ].
   destruct_conjs.
   eexists; split; [eassumption|].
   intros.
-  assert (exists elem_rel : relation (domain P), rel_typ_unsorted pred_P A ρ A ρ' elem_rel) by mauto.
+  assert (exists elem_rel : relation (domain P), rel_typ_unsorted pred_P Δ A ρ A ρ' elem_rel) by mauto.
   destruct_conjs.
   destruct_by_head (@rel_typ_unsorted).
   eexists; econstructor; mauto.
@@ -386,16 +391,16 @@ Qed.
 Hint Resolve rel_typ_sub_id : mcpts.
 
 
-Lemma rel_typ_sym {P} {pred_P : PredicativeSig P} {Γ A B} :
-  {{ ⟪ pred_P ⟫ Γ ⊨ A ≈ B }} ->
-  {{ ⟪ pred_P ⟫ Γ ⊨ B ≈ A }}.
+Lemma rel_typ_sym {P} {pred_P : PredicativeSig P} {Δ Γ A B} :
+  {{ ⟪ pred_P ⟫ Δ ▶ Γ ⊨ A ≈ B }} ->
+  {{ ⟪ pred_P ⟫ Δ ▶ Γ ⊨ B ≈ A }}.
 Proof.
   intros * [env_relΓ].
   destruct_conjs.
   eexists; split; [eassumption |].
   intros.
   symmetry in equiv_ρ_ρ'.
-  assert (exists elem_rel : relation (domain P), rel_typ_unsorted pred_P A ρ' B ρ elem_rel) by mauto.
+  assert (exists elem_rel : relation (domain P), rel_typ_unsorted pred_P Δ A ρ' B ρ elem_rel) by mauto.
   destruct_conjs.
   destruct_by_head (@rel_typ_unsorted P).
   exists H1.
@@ -407,10 +412,10 @@ Qed.
 #[export]
 Hint Resolve rel_typ_sym : mcpts.
 
-Lemma rel_typ_trans {P} {pred_P : PredicativeSig P} {Γ A1 A2 A3} :
-  {{ ⟪ pred_P ⟫ Γ ⊨ A1 ≈ A2 }} ->
-  {{ ⟪ pred_P ⟫ Γ ⊨ A2 ≈ A3 }} ->
-  {{ ⟪ pred_P ⟫ Γ ⊨ A1 ≈ A3 }}.
+Lemma rel_typ_trans {P} {pred_P : PredicativeSig P} {Δ Γ A1 A2 A3} :
+  {{ ⟪ pred_P ⟫ Δ ▶ Γ ⊨ A1 ≈ A2 }} ->
+  {{ ⟪ pred_P ⟫ Δ ▶ Γ ⊨ A2 ≈ A3 }} ->
+  {{ ⟪ pred_P ⟫ Δ ▶ Γ ⊨ A1 ≈ A3 }}.
 Proof.
   intros * [env_relΓ] [env_relΓ'].
   destruct_conjs.
@@ -419,8 +424,8 @@ Proof.
   eexists; split; [eassumption|].
   intros.
   assert (equiv_ρ_ρ : env_relΓ ρ ρ) by (etransitivity; [|symmetry]; eassumption).
-  assert (exists elem_rel : relation (domain P), rel_typ_unsorted pred_P A1 ρ A2 ρ elem_rel) by mauto.
-  assert (exists elem_rel : relation (domain P), rel_typ_unsorted pred_P A2 ρ A3 ρ' elem_rel) by mauto.
+  assert (exists elem_rel : relation (domain P), rel_typ_unsorted pred_P Δ A1 ρ A2 ρ elem_rel) by mauto.
+  assert (exists elem_rel : relation (domain P), rel_typ_unsorted pred_P Δ A2 ρ A3 ρ' elem_rel) by mauto.
   destruct_conjs.
   destruct_by_head (@rel_typ_unsorted).
   handle_per_typ_elem_irrel.
@@ -432,17 +437,17 @@ Qed.
 Hint Resolve rel_typ_trans : mcpts.
 
 #[export]
-Instance rel_typ_under_ctx_PER {P : PtsSig} {pred_P : PredicativeSig P} {Γ} : PER (rel_typ_under_ctx pred_P Γ).
+Instance rel_typ_under_ctx_PER {P : PtsSig} {pred_P : PredicativeSig P} {Δ Γ} : PER (rel_typ_under_ctx pred_P Δ Γ).
 Proof.
   split; mauto.
 Qed.
 
-Lemma presup_rel_exp {P : PtsSig} {pred_P : PredicativeSig P} : forall {Γ M M' A},
-    {{ ⟪ pred_P ⟫ Γ ⊨u M ≈ M' : A }} ->
-    {{ ⟪ pred_P ⟫ ⊨ Γ }} /\ {{ ⟪ pred_P ⟫ Γ ⊨u M : A }} /\ {{ ⟪ pred_P ⟫ Γ ⊨u M' : A }} /\ {{ ⟪ pred_P ⟫ Γ ⊨ A }}.
+Lemma presup_rel_exp {P : PtsSig} {pred_P : PredicativeSig P} : forall {Δ Γ M M' A},
+    {{ ⟪ pred_P ⟫ Δ ▶ Γ ⊨u M ≈ M' : A }} ->
+    {{ ⟪ pred_P ⟫ Δ ▶ Γ }} /\ {{ ⟪ pred_P ⟫ Δ ▶ Γ ⊨u M : A }} /\ {{ ⟪ pred_P ⟫ Δ ▶ Γ ⊨u M' : A }} /\ {{ ⟪ pred_P ⟫ Δ ▶ Γ ⊨ A }}.
 Proof.
   intros *.
-  assert (Hpart : {{ ⟪ pred_P ⟫ Γ ⊨u M ≈ M' : A }} -> {{ ⟪ pred_P ⟫ Γ ⊨u M : A }} /\ {{ ⟪ pred_P ⟫ Γ ⊨u M' : A }}) by (split; unfold valid_exp_under_ctx_unsorted; etransitivity; [|symmetry|symmetry|]; eassumption).
+  assert (Hpart : {{ ⟪ pred_P ⟫ Δ ▶ Γ ⊨u M ≈ M' : A }} -> {{ ⟪ pred_P ⟫ Δ ▶ Γ ⊨u M : A }} /\ {{ ⟪ pred_P ⟫ Δ ▶ Γ ⊨u M' : A }}) by (split; unfold valid_exp_under_ctx_unsorted; etransitivity; [|symmetry|symmetry|]; eassumption).
   intros Hrel; repeat split;
     try solve [intuition]; clear Hpart;
     destruct Hrel as [env_relΓ];
@@ -459,10 +464,10 @@ Qed.
 #[export]
 Hint Resolve presup_rel_exp : mcpts.
 
-Lemma rel_exp_eq_subtyp{P : PtsSig} {pred_P : PredicativeSig P} : forall Γ M M' A A',
-    {{ ⟪ pred_P ⟫ Γ ⊨u M ≈ M' : A }} ->
-    {{ ⟪ pred_P ⟫ Γ ⊨ A ⊆ A' }} ->
-    {{ ⟪ pred_P ⟫ Γ ⊨u M ≈ M' : A' }}.
+Lemma rel_exp_eq_subtyp{P : PtsSig} {pred_P : PredicativeSig P} : forall Δ Γ M M' A A',
+    {{ ⟪ pred_P ⟫ Δ ▶ Γ ⊨u M ≈ M' : A }} ->
+    {{ ⟪ pred_P ⟫ Δ ▶ Γ ⊨ A ⊆ A' }} ->
+    {{ ⟪ pred_P ⟫ Δ ▶ Γ ⊨u M ≈ M' : A' }}.
 Proof.
   intros * HM [env_relΓ [? ?]].
   invert_rel_exp_unsorted HM.
@@ -476,7 +481,7 @@ Proof.
   split; econstructor; eauto using per_sort_elem_cumu.
   handle_per_sort_elem_irrel.
   eapply per_elem_subtyping_gen; [| | | try eassumption].
-  - eauto using per_subtyp_sorted_cumu.
+  - eauto.
   - eauto using per_sort_elem_cumu.
   - symmetry.
     eauto using per_sort_elem_cumu.
